Agreement proof overhaul

paxos/proof.dfy
@@ -108,18 +108,10 @@ predicate Agreement(c:Constants, ds:DistrSys)
     requires c.WF()
     requires ds.WF(c)
 {
-    forall v, b, idx | c.ValidLdrIdx(idx) && LeaderIdxDecidedV(c, ds, idx, v, b) 
-    :: AllDecidedProcessesDecidesV(c, ds, v)
-}
-
-predicate LeaderIdxDecidedV(c:Constants, ds:DistrSys, idx:int, v:Value, b:Ballot) 
-    requires c.WF() && ds.WF(c)
-    requires c.ValidLdrIdx(idx)
-{
-    && b != Bottom
-    && ds.leaders[idx].state == Decided 
-    && ds.leaders[idx].val == v
-    && ds.leaders[idx].ballot == b
+    forall i1, i2 | 
+        && c.ValidLdrIdx(i1) && LeaderHasDecided(c, ds, i1) 
+        && c.ValidLdrIdx(i2) && LeaderHasDecided(c, ds, i2) 
+    :: TwoLeadersHaveSameV(c, ds, i1, i2)
 }
 
 
@@ -130,16 +122,125 @@ predicate Agreement_Inv(c:Constants, ds:DistrSys)
     && ds.WF(c)
     && Agreement(c, ds)
     && LdrBallotNotBottom(c, ds)
-    && Agreement_Inv_Lemma(c, ds)
+    && LdrAcceptsSetUnique(c, ds)
+    && LdrAcceptsSetCorrespondToAcceptMsg(c, ds)
+    && LdrPromisesSetUnique(c, ds)
+    && LdrPromisesSetCorrespondToPromiseMsg(c, ds)
+    && (forall i | c.ValidLdrIdx(i) && LeaderHasDecided(c, ds, i) 
+        :: Agreement_Inv_Decided(c, ds, i)
+    )
 }
 
+/* All l.accepts collected by l are unique source */
+predicate LdrAcceptsSetUnique(c:Constants, ds:DistrSys) 
+    requires c.WF() && ds.WF(c)
+{
+    forall i | c.ValidLdrIdx(i) ::(
+        forall s1, s2 | s1 in ds.leaders[i].accepts && s2 in ds.leaders[i].accepts 
+        :: s1 != s2
+    )
+}
+
+/* All l.accepts collected by l came from network */
+predicate LdrAcceptsSetCorrespondToAcceptMsg(c:Constants, ds:DistrSys) 
+    requires c.WF() && ds.WF(c)
+{
+    forall i | c.ValidLdrIdx(i) ::(
+        forall s | s in ds.leaders[i].accepts
+        :: Packet(s, Id(Ldr, i), Accept(ds.leaders[i].ballot)) in ds.network.sentPackets
+    )
+}
+
+/* All l.promises collected by l are unique source */
+predicate LdrPromisesSetUnique(c:Constants, ds:DistrSys) 
+    requires c.WF() && ds.WF(c)
+{
+    forall i | c.ValidLdrIdx(i) ::(
+        forall p1, p2 | p1 in ds.leaders[i].promises && p2 in ds.leaders[i].promises 
+        :: p1.src != p2.src
+    )
+}
+
+/* All l.promises collected by l came from network */
+predicate LdrPromisesSetCorrespondToPromiseMsg(c:Constants, ds:DistrSys) 
+    requires c.WF() && ds.WF(c)
+{
+    forall i | c.ValidLdrIdx(i) ::(
+        forall p | p in ds.leaders[i].promises
+        :: p in ds.network.sentPackets
+    )
+}
 
 predicate LdrBallotNotBottom(c:Constants, ds:DistrSys) 
     requires c.WF() && ds.WF(c)
 {
     && (forall l | l in ds.leaders :: l.ballot != Bottom)
-    // && (forall m | m in ds.network.sentPackets ::
 }
+
+/* Things that are true if v is decided with ballot b. */
+predicate Agreement_Inv_Decided(c:Constants, ds:DistrSys, i:int) 
+    requires c.WF() && ds.WF(c)
+    requires c.ValidLdrIdx(i) && LeaderHasDecided(c, ds, i) 
+{
+    var b, v := ds.leaders[i].ballot, ds.leaders[i].val;
+    && LargerBallotPhase2LeadersV(c, ds, v, b)
+    && LargerBallotAcceptors(c, ds, v, b)
+    && LargerBallotPromiseMsgs(c, ds, v, b)
+    && LargerBallotProposeMsgs(c, ds, v, b)
+    && LargerBallotsPromiseQrms(c, ds, v, b)
+}
+
+/* If v is decided with ballot b, then all phase 2 leaders with ballots
+* b' >= b must be of v */
+predicate LargerBallotPhase2LeadersV(c:Constants, ds:DistrSys, v:Value, b:Ballot) 
+    requires c.WF() && ds.WF(c)
+{
+    forall i' | 
+        && c.ValidLdrIdx(i') 
+        && BalLtEq(b, ds.leaders[i'].ballot) 
+        && LeaderInPhase2(c, ds, i') 
+    :: LeaderHasValueV(c, ds, i', v)
+}
+
+/* If v is decided with ballot b, then for any acceptor that accepted a ballot b'>=b, 
+* the accepted value is v */
+predicate LargerBallotAcceptors(c:Constants, ds:DistrSys, v:Value, b:Ballot) 
+    requires c.WF() && ds.WF(c)
+{
+    forall i' | c.ValidAccIdx(i') && BalLtEq(b, ds.acceptors[i'].accepted.b)
+    :: AcceptorHasValueV(c, ds, i', v)
+}
+
+
+/* If v is decided with ballot b, then for any Promise msgs with valbal ballot b'>=b, 
+* the valbal value is v */
+predicate LargerBallotPromiseMsgs(c:Constants, ds:DistrSys, v:Value, b:Ballot) 
+    requires c.WF() && ds.WF(c)
+{
+    forall p | p in ds.network.sentPackets && p.msg.Promise? && BalLtEq(b, p.msg.vb.b)
+    :: p.msg.vb.v == v
+}
+
+/* If v is decided with ballot b, then for any Propose msgs with ballot b'>=b, 
+* the value is v */
+predicate LargerBallotProposeMsgs(c:Constants, ds:DistrSys, v:Value, b:Ballot) 
+    requires c.WF() && ds.WF(c)
+{
+    forall p | p in ds.network.sentPackets && p.msg.Propose? && BalLtEq(b, p.msg.bal)
+    :: p.msg.val == v
+}
+
+/* If v is decided with ballot b, then all Promise quorums for ballots
+* b' >= b must come from an acceptor that accepted (v, b) */
+predicate LargerBallotsPromiseQrms(c:Constants, ds:DistrSys, v:Value, b:Ballot) 
+    requires c.WF() && ds.WF(c)
+{
+    forall b' | BalLtEq(b, b') 
+    :: (forall qrm:set<Packet> | QuorumOfPromiseMsgs(c, ds, qrm, b') 
+        :: exists p :: p in qrm && BalLtEq(b, p.msg.vb.b) 
+    )
+}
+
 
 
 /* Init ==> Agreement_Inv */
@@ -155,359 +256,16 @@ lemma NextPreservesAgreementInv(c:Constants, ds:DistrSys, ds':DistrSys)
     requires Next(c, ds, ds')
     ensures Agreement_Inv(c, ds')
 {
-
-    if exists v, b, i :: c.ValidLdrIdx(i) && LeaderIdxDecidedV(c, ds, i, v, b) {
-        // If someone has decided in ds
-        NextPreservesAgreementInv_Case_ExistingDecision(c, ds, ds');
-    } else {
-        // If no one has decided in ds
-        NextPreservesAgreementInv_Case_NoExistingDecision(c, ds, ds');
-    }
-}
-
-lemma NextPreservesAgreementInv_Case_ExistingDecision(c:Constants, ds:DistrSys, ds':DistrSys) 
-    requires Agreement_Inv(c, ds)
-    requires Next(c, ds, ds')
-    requires exists v, b, i :: c.ValidLdrIdx(i) && LeaderIdxDecidedV(c, ds, i, v, b)
-    ensures Agreement_Inv(c, ds')
-{
-    NextPreservesAgreementInvLemma(c, ds, ds');
-    var v, b, i :| c.ValidLdrIdx(i) && LeaderIdxDecidedV(c, ds, i, v, b);
-    var actor, recvIos:seq<Packet>, sendIos:seq<Packet> :| PaxosNextOneAgent(c, ds, ds', actor, recvIos, sendIos);
-    if actor.agt.Ldr? {
-        var l, l' := ds.leaders[actor.idx], ds'.leaders[actor.idx];
-        if l.state == P2b && recvIos[0].msg.Accept? {
-            var src, msg := recvIos[0].src, recvIos[0].msg;
-            if msg.bal == l.ballot && src !in l.accepts && |l.accepts| == 2*l.consts.f {
-                var b', v' := l.ballot, l.val;
-                if v' != v {
-                    assert LeaderIdxDecidedV(c, ds', actor.idx, v', b'); 
-                    assert LeaderIdxDecidedV(c, ds', i, v, b); 
-                    if BalLtEq(b, b'){
-                        assert false;
-                    } else {
-                        assert BalLtEq(b', b);
-                        assert false;
-                    }
-                }
-            }
-        } 
-    }
-}
-
-lemma NextPreservesAgreementInv_Case_NoExistingDecision(c:Constants, ds:DistrSys, ds':DistrSys) 
-    requires Agreement_Inv(c, ds)
-    requires Next(c, ds, ds')
-    requires forall v, b, i | c.ValidLdrIdx(i) :: !LeaderIdxDecidedV(c, ds, i, v, b)
-    ensures Agreement_Inv(c, ds')
-{
-    NextPreservesAgreementInvLemma(c, ds, ds');
-    var src, recvIos, sendIos :| PaxosNextOneAgent(c, ds, ds', src, recvIos, sendIos);
-    forall l | l in ds.leaders 
-    ensures !l.state.Decided? {
-        if l.state.Decided? {
-            var v, b, i := l.val, l.ballot, l.consts.id.idx;
-            assert b != Bottom;
-            assert LeaderIdxDecidedV(c, ds, i, v, b);
-            assert false;
-        }
-    }
-}
-
-
-///////////////////////          Agreement Sub-Lemma         /////////////////////////////
-
-
-predicate Agreement_Inv_Lemma(c:Constants, ds:DistrSys) 
-{
-    && c.WF()
-    && ds.WF(c)
-    && LeaderPromisesSetProperty(c, ds)
-    && Agreement_Safey(c, ds)
-    && (forall v, b, i | c.ValidLdrIdx(i) && LeaderIdxDecidedV(c, ds, i, v, b) 
-        :: AgreementInvProperties_Decided(c, ds, v, b))
-}
-
-predicate Agreement_Safey(c:Constants, ds:DistrSys) 
-    requires c.WF() && ds.WF(c)
-{
-    forall v, b, i | c.ValidLdrIdx(i) && LeaderIdxDecidedV(c, ds, i, v, b)
-    :: LargerBallotsDecideV(c, ds, v, b)
-}
-
-predicate AgreementInvProperties_Decided(c:Constants, ds:DistrSys, v:Value, b:Ballot)
-    requires c.WF() && ds.WF(c)
-{
-    && v != Nil
-    && LargerBallotsPromiseQrms(c, ds, v, b)
-    && LargerBallotPhase2LeadersV(c, ds, v, b)
-    && LargerBallotAcceptors(c, ds, v, b)
-    && LargerBallotPromiseMsgs(c, ds, v, b)
-    && LargerBallotProposalMsgs(c, ds, v, b)
-}
-
-
-predicate LeaderPromisesSetProperty(c:Constants, ds:DistrSys) 
-    requires c.WF() && ds.WF(c)
-{
-    forall i | c.ValidLdrIdx(i) :: (
-        forall p | p in ds.leaders[i].promises :: 
-            && p in ds.network.sentPackets
-            && p.msg.Promise?
-            && p.msg.bal == ds.leaders[i].ballot
-    )
-}
-
-
-/* If v is decided with ballot b, then all values decided with ballots
-* b' >= b must be of v */
-predicate LargerBallotsDecideV(c:Constants, ds:DistrSys, v:Value, b:Ballot)
-    requires c.WF() && ds.WF(c)
-{
-    forall b', i' | 
-        && c.ValidLdrIdx(i') && BalLtEq(b, b') 
-        && LeaderHasDecided(c, i', ds) && LeaderHasBallotB(c, i', ds, b') 
-    :: LeaderHasValueV(c, i', ds, v)
-}
-
-
-/* If v is decided with ballot b, then all Promise quorums for ballots
-* b' >= b must come from an acceptor that accepted (v, b) */
-predicate LargerBallotsPromiseQrms(c:Constants, ds:DistrSys, v:Value, b:Ballot) 
-    requires c.WF() && ds.WF(c)
-{
-    forall b' | BalLtEq(b, b') 
-    :: (forall qrm:set<Packet> | QuorumOfPromiseMsgs(c, ds, qrm, b') 
-        :: exists p :: p in qrm && BalLtEq(b, p.msg.vb.b) 
-    )
-}
-
-/* If v is decided with ballot b, then all phase 2 leaders with ballots
-* b' >= b must be of v */
-predicate LargerBallotPhase2LeadersV(c:Constants, ds:DistrSys, v:Value, b:Ballot) 
-    requires c.WF() && ds.WF(c)
-{
-    forall b', i' | 
-        && c.ValidLdrIdx(i') && BalLtEq(b, b') 
-        && LeaderInPhase2(c, i', ds) && LeaderHasBallotB(c, i', ds, b')
-    :: LeaderHasValueV(c, i', ds, v)
-}
-
-/* If v is decided with ballot b, then there is a quorum q of acceptors such that all in q
-* accepted b' >= b with value v */
-predicate QuorumOfAcceptorsAcceptedBV(c:Constants, ds:DistrSys, q:set<int>, v:Value, b:Ballot) 
-    requires c.WF() && ds.WF(c)
-    requires QuorumOfAcceptors(c, q)
-{
-    forall idx | idx in q ::
-        && ds.acceptors[idx].accepted.v == v
-        && BalLtEq(b, ds.acceptors[idx].accepted.b)
-}
-
-/* If v is decided with ballot b, then for any acceptor that accepted a ballot b'>=b, 
-* the accepted value is v */
-predicate LargerBallotAcceptors(c:Constants, ds:DistrSys, v:Value, b:Ballot) 
-    requires c.WF() && ds.WF(c)
-{
-    forall idx | c.ValidAccIdx(idx) && BalLtEq(b, ds.acceptors[idx].accepted.b)
-    :: ds.acceptors[idx].accepted.v == v
-}
-
-/* If v is decided with ballot b, then for any Promise msgs with valbal ballot b'>=b, 
-* the valbal value is v */
-predicate LargerBallotPromiseMsgs(c:Constants, ds:DistrSys, v:Value, b:Ballot) 
-    requires c.WF() && ds.WF(c)
-{
-    forall p | p in ds.network.sentPackets && p.msg.Promise? && BalLtEq(b, p.msg.vb.b)
-    :: p.msg.vb.v == v
-}
-
-/* If v is decided with ballot b, then for any Proposal msgs with ballot b'>=b, 
-* the value is v */
-predicate LargerBallotProposalMsgs(c:Constants, ds:DistrSys, v:Value, b:Ballot) 
-    requires c.WF() && ds.WF(c)
-{
-    forall p | p in ds.network.sentPackets && p.msg.Propose? && BalLtEq(b, p.msg.bal)
-    :: p.msg.val == v
-}
-
-
-/* Main theorem for Agreement_Inv_Lemma */
-lemma NextPreservesAgreementInvLemma(c:Constants, ds:DistrSys, ds':DistrSys) 
-    requires Agreement_Inv_Lemma(c, ds)
-    requires Next(c, ds, ds')
-    ensures Agreement_Inv_Lemma(c, ds')
-{
-    if exists v, b, i :: c.ValidLdrIdx(i) && LeaderIdxDecidedV(c, ds, i, v, b) {
-        var v, b, i :| c.ValidLdrIdx(i) && LeaderIdxDecidedV(c, ds, i, v, b);
-        NextPreservesAgreementInvLemma_1(c, ds, ds', i, v, b);
-    } else {
+    if SomeLeaderHasDecided(c, ds) {
+        var i1 :| c.ValidLdrIdx(i1) && LeaderHasDecided(c, ds, i1);
+        // TODO
         assume false;
+        assert Agreement_Inv(c, ds');
+    } else {
+        // TODO
+        assume false;
+        assert Agreement_Inv(c, ds');
     }
 }
-
-
-lemma NextPreservesAgreementInvLemma_1(c:Constants, ds:DistrSys, ds':DistrSys, i:int, v:Value, b:Ballot) 
-    requires Agreement_Inv_Lemma(c, ds)
-    requires Next(c, ds, ds')
-    requires c.ValidLdrIdx(i) && LeaderIdxDecidedV(c, ds, i, v, b);
-    ensures Agreement_Inv_Lemma(c, ds')
-{   
-    forall v', b', i' | c.ValidLdrIdx(i') && LeaderIdxDecidedV(c, ds', i', v', b')
-    ensures && LargerBallotsDecideV(c, ds', v', b')
-            && AgreementInvProperties_Decided(c, ds', v', b');
-    {
-        if BalLtEq(b, b') {
-            assert v' == v;
-
-            forall bx | BalLtEq(b', bx) 
-            ensures forall qrm:set<Packet> | QuorumOfPromiseMsgs(c, ds', qrm, bx) 
-                    :: exists p :: p in qrm && BalLtEq(b', p.msg.vb.b) 
-            {
-                forall qrm:set<Packet> | QuorumOfPromiseMsgs(c, ds', qrm, bx) 
-                ensures exists p :: p in qrm && BalLtEq(b', p.msg.vb.b) 
-                {
-                    assert exists p :: p in qrm && BalLtEq(b', p.msg.vb.b);
-                }
-            }
-            assert LargerBallotsPromiseQrms(c, ds', v', b');
-
-            forall bx, ix | 
-                && c.ValidLdrIdx(ix) && BalLtEq(b, bx) 
-                && LeaderInPhase2(c, ix, ds') && LeaderHasBallotB(c, ix, ds', bx)
-            ensures LeaderHasValueV(c, ix, ds', v)
-            {
-                if !LeaderInPhase2(c, ix, ds) {
-                    var actor, recvIos:seq<Packet>, sendIos :| PaxosNextOneAgent(c, ds, ds', actor, recvIos, sendIos);
-                    if actor.agt == Ldr {
-                        var l, l' := ds.leaders[actor.idx], ds'.leaders[actor.idx];
-                        if l.state == P1b && recvIos[0].msg.Promise? {
-                            var src, msg := recvIos[0].src, recvIos[0].msg;
-                            if msg.bal == l.ballot && !exists p :: p in l.promises && p.src == src {
-                                if |l.promises| == 2*l.consts.f{
-                                    var qrm := l.promises + {recvIos[0]};
-                                    assert QuorumOfPromiseMsgs(c, ds, qrm, l.ballot);
-                                    assert exists p :: p in qrm && BalLtEq(b, p.msg.vb.b);
-                                }
-                            }
-                        } 
-                    }
-                }
-            }
-            assert AgreementInvProperties_Decided(c, ds', v', b');  // Inv
-            
-            forall bx, ix | 
-                && c.ValidLdrIdx(ix) && BalLtEq(b', bx) 
-                && LeaderHasDecided(c, ix, ds') && LeaderHasBallotB(c, ix, ds', bx) 
-            ensures LeaderHasValueV(c, ix, ds', v)
-            {
-                // TODO: This one is def true, but fragile. Dafny sees it sometimes, but sometimes not.
-                assert LargerBallotsPromiseQrms(c, ds, v, b);
-            }
-            assert LargerBallotsDecideV(c, ds', v', b');    // Safety
-        } else {
-            // TODO
-            assume false;
-        }
-    }
-    assert Agreement_Inv_Lemma(c, ds');
-}
-
-
-
-
-lemma Lemma_LargerBallotAcceptors_1(c:Constants, ds:DistrSys, ds':DistrSys,i:int, v:Value, b:Ballot) 
-    requires Agreement_Inv_Lemma(c, ds)
-    requires Next(c, ds, ds')
-    requires c.ValidLdrIdx(i) && LeaderIdxDecidedV(c, ds, i, v, b)
-    ensures LargerBallotAcceptors(c, ds', v, b)
-{}
-
-lemma Lemma_LargerBallotsDecideV_1(c:Constants, ds:DistrSys, ds':DistrSys,i:int, v:Value, b:Ballot) 
-    requires Agreement_Inv_Lemma(c, ds)
-    requires Next(c, ds, ds')
-    requires c.ValidLdrIdx(i) && LeaderIdxDecidedV(c, ds, i, v, b)
-    ensures LargerBallotsDecideV(c, ds', v, b)
-{}
-
-// lemma Lemma_LargerBallotPhase2LeadersV_1(c:Constants, ds:DistrSys, ds':DistrSys,i:int, v:Value, b:Ballot) 
-//     requires Agreement_Inv_Lemma(c, ds)
-//     requires Next(c, ds, ds')
-//     requires c.ValidLdrIdx(i) && LeaderIdxDecidedV(c, ds, i, v, b)
-//     ensures LargerBallotPhase2LeadersV(c, ds', v, b)
-// {
-//     var actor, recvIos:seq<Packet>, sendIos :| PaxosNextOneAgent(c, ds, ds', actor, recvIos, sendIos);
-//     if actor.agt == Ldr {
-//         var l, l' := ds.leaders[actor.idx], ds'.leaders[actor.idx];
-//         if l.state == P1b && BalLtEq(b, l.ballot) {
-//             var pkt := recvIos[0];
-//             if pkt.msg.Promise? {
-//                 var src, msg := pkt.src, pkt.msg;
-//                 if  && msg.bal == l.ballot 
-//                     && (!exists p :: p in l.promises && p.src == src) 
-//                     && |l.promises| == 2*l.consts.f 
-//                 {
-//                     var qrm := l.promises + {pkt};
-//                     assert QuorumOfPromiseMsgs(c, ds, qrm, l.ballot);
-//                     assert PromiseWithHighestBallot(qrm).v == v;
-//                     assert LargerBallotPhase2LeadersV(c, ds', v, b);
-//                 }
-//             }
-//         }
-//     }
-// }
-
-
-
-
-
-// predicate Agreement_Inv_AcceptedByQuorum(c:Constants, ds:DistrSys, v:Value, b:Ballot) 
-//     requires c.WF() && ds.WF(c)
-// {
-//     SomeProcessDecidedV(c, ds, v, b) ==> (
-//         exists quorum ::
-//             && QuorumOfAcceptors(c, quorum)
-//             && AcceptedByQuroum(c, ds, quorum, v, b)
-//     )
-// }
-
-// predicate AcceptedByQuroum(c:Constants, ds:DistrSys, q:set<int>, v:Value, b:Ballot) 
-//     requires c.WF() && ds.WF(c)
-//     requires QuorumOfAcceptors(c, q)
-// {
-//     forall idx | idx in q ::
-//         && ds.acceptors[idx].accepted == v
-//         && BalLtEq(b, ds.acceptors[idx].promised)
-// }
-
-
-// predicate Agreement_Inv_Messages(c:Constants, ds:DistrSys, v:Value, b:Ballot) 
-//     requires c.WF() && ds.WF(c)
-// {
-//     SomeProcessDecidedV(c, ds, v, b) 
-//     ==> 
-//     (forall pkt | pkt in ds.network.sentPackets && BalLtEq(b, pkt.msg.bal)
-//     :: ProposeAndPreemptContainsV(pkt.msg, v))
-// }
-
-// predicate ProposeAndPreemptContainsV(m:Message , v:Value) {
-//     match m {
-//         case Propose(bal, val) => val == v
-//         case Preempt(bal, val) => val == v
-//         case _ => true
-//     }
-// }
-
-// predicate Agreement_Inv_P2Leaders(c:Constants, ds:DistrSys, v:Value, b:Ballot) 
-//     requires c.WF() && ds.WF(c)
-// {
-//     SomeProcessDecidedV(c, ds, v, b) 
-//     ==> 
-//     (forall i | 
-//         && c.ValidLdrIdx(i) 
-//         && LeaderInPhase2(c, i, ds) 
-//         && BalLtEq(b, ds.leaders[i].ballot)
-//     :: ds.leaders[i].val == v)
-// }
 
 }
